\documentclass[12pt]{report}

\usepackage[utf8]{inputenc}
\usepackage{amsmath}
\usepackage{amsthm}
\usepackage{amssymb}
\usepackage{amsfonts}
\usepackage{graphics}

\begin{document}

%%%%%%%%%%%%%%%%%%%%%%%%%%%%%%%%%%%%%%%%%%%%%%%%%%%%%%%%%%%%%%%%%%%%%%%%%%%%%
\subsection{Lag-One Covariance Smoother}

In order to estimate $A$ and $Q$, we need to calculate $P_{t,t-1}^t$. Let's
define $\tilde{x_t^s} = x_t - \hat{x}_t^s$. Then,

\begin{eqnarray*}
P_{t,t-1}^t &=& E ( \tilde{x}_t^t \tilde{x}{_{t-1}^t}'  ) \\
&=& E[ (x_t - \hat{x}_t^t) (x_{t-1} - \hat{x}_{t-1}^t)' ]
\end{eqnarray*}

\begin{eqnarray*}
x_{t-1}' = x_{t-1}^{t-1} + L_{t-1} (x' - x_t ^ {t-1}) \\
x_{t-1}^t = x_{t-1}^{t-1} + L_{t-1} (x^t - x_t ^ {t-1}) 
\end{eqnarray*}

\begin{eqnarray*}
x_t^t = x_t^{t-1} + K_t(y_t - Cx_t^{t-1}) \\
x_t^t - x_t^{t-1} = K_t(y_t - Cx_t^{t-1})
\end{eqnarray*}

\begin{eqnarray*}
P_{t,t-1} &=& E\bigg[
  (x_t - x_t^{t-1} - K_t(y_t - Cx_t^{t-1}) )
  (x_{t-1} - x_{t-1}^{t-1} - J_{t-1}(x_t^t - x_t^{t-1}))'
  \bigg]\\
&=& E\bigg[
  (x_t - x_t^{t-1} - K_t(y_t - Cx_t^{t-1}))
  (x_{t-1} - x_{t-1}^{t-1} - J_{t-1}K_t(y_t - Cx_t^{t-1}))'
  \bigg]\\
&=& E\bigg[
  (\tilde{x}_t^{t-1} - K_t(y_t - Cx_t^{t-1}))
  (\tilde{x}_{t-1}^{t-1} - J_{t-1}K_t(y_t - Cx_t^{t-1}))'
  \bigg]
\end{eqnarray*}

\begin{eqnarray*}
y_t &=& Cx_t + v_t \\
&=& Cx_t - Cx_t^{t-1} - v_t \\
&=& C(x_t - x_t^{t-1})+v_t \\
&=& C\tilde{x}_t^{t-1}+v_t
\end{eqnarray*}

\begin{eqnarray*}
P_{t,t-1}^t &=& E\bigg[
  (\tilde{x}_t^{t-1} - K_t( C\tilde{x}_t^{t-1}+v_t ))
  (\tilde{x}_{t-1}^{t-1} - J_{t-1}K_t( C\tilde{x}_t^{t-1}+v_t ))' 
  \bigg]
\end{eqnarray*}

\begin{eqnarray}
&=& E\bigg[
  \tilde{x}_t^{t-1}\tilde{x}{_{t-1}^{t-1}}' \label{exp1} \\
&& -
  \tilde{x}_t^{t-1}(L_{t-1}K_t(Cx_t^{t-1}+v_t))' \label{exp2} \\
&& -
  K_t(C\tilde{x}_t^{t-1}+v_t)\tilde{x}{_{t-1}^{t-1}}' \label{exp3}  \\
&& +
  K_t(C\tilde{x}_t^{t-1}+v_t)(L_{t-1}K_t(C\tilde{x}_t^{t-1}+ v_t))' \label{exp4} \bigg]
\end{eqnarray}

\begin{eqnarray*}
E[\tilde{x}_t^{t-1}\tilde{x}{_{t-1}^{t-1}}'] &=& P_{t,t-1}^{t-1}
\end{eqnarray*}

\begin{eqnarray*}
  &=& -E[ \tilde{x}_t^{t-1}(L_{t-1}K_t(Cx_t^{t-1}+v_t))' ] \\
  &=& -E[\tilde{x}_t^{t-1}(\tilde{x}{_t^{t-1}}'C' + v_t') L_{t-1}' K_t'] \\
  &=& -E[\tilde{x}_t^{t-1}\tilde{x}{_t^{t-1}}'C' + \tilde{x}_t^{t-1}v_t'] \\
  &=& -P_t^{t-1}C'K_t'L_{t-1}'
\end{eqnarray*}

\begin{eqnarray*}
  &=& -E[K_t(C\tilde{x}_t^{t-1}+v_t)\tilde{x}{_{t-1}^{t-1}}' ] \\
  &=& -E[K_tC\tilde{x}_t^{t-1}\tilde{x}{_{t-1}^{t-1}}' + K_tv_t\tilde{x}{_{t-1}^{t-1}}']\\
  &=& -E[K_tC\tilde{x}_t^{t-1}\tilde{x}{_{t-1}^{t-1}}']\\
  &=& -K_tCP_{t,t-1}^{t-1}
\end{eqnarray*}


\begin{eqnarray*}
  &=& E[(K_t C \tilde{x}_t^{t-1} + v_t)(L_{t-1}K_t(C\tilde{x}_t^{t-1}+ v_t))']\\
  &=& E[(K_tC\tilde{x}_t^{t-1} + K_tv_t) 
    [ \tilde{x}{_t^{t-1}}' C' K_t' L_{t-1}' + v_t' K_t'L_{t-1}'] ] \\
  &=& E[K_t C \tilde{x}_t^{t-1} \tilde{x}{_t^{t-1}}' C' K_t' L_{t-1}' +
    K_tv_t v_t' K_t'L_{t-1}' + ... ]\\
  &=& K_tCP_t^{t-1}C'Kt'L_{t-1}' + K_t\Sigma_wK_t'L_{t-1}T\\
  &=& K_t(CP_t^{t-1}C' + \Sigma_w)K_t'L_{t-1}'
\end{eqnarray*}

Based on the definition of $K_t$ 
\begin{eqnarray*}
K_t &=& P_{t}^{t-1}C' (CP_{t}^tC'+ \Sigma_{w})^{-1}\\
K_t (CP_{t}^tC'+ \Sigma_{w}) &=& P_{t}^{t-1} C'
\end{eqnarray*}

Hence we can continue with previous Equation as

\begin{eqnarray*}
  &=& P_{t}^{t-1} C' K_t'L_{t-1}'
\end{eqnarray*}

The full equation is

\begin{eqnarray*}
P_{t,t-1}^t = P_{t,t-1}^{t-1} - P_t^{t-1}C'K_t'L_{t-1}' - K_tCP_{t,t-1}^{t-1} + P_{t}^{t-1} C' K_t'L_{t-1}'
\end{eqnarray*}

If we remember the joint covariance of joint distribution $(x_{t},x_{t-1})$ is
$AP_{t-1}^{t-1}$ (we simply look at the lower left cell of covariance matrix for
$(x_{t-1},x_{t})$), this means $P_{t,t-1}^{t-1} = AP_{t-1}^{t-1}$, then

\begin{eqnarray*}
  P_{t,t-1}^t &=& AP_{t-1}^{t-1} - P_t^{t-1}C'K_t'L_{t-1}' - K_t C AP_{t-1}^{t-1} + P_{t}^{t-1} C' K_t'L_{t-1}'\\
  &=& AP_{t-1}^{t-1}  - K_t C AP_{t-1}^{t-1} \\
  &=& (I  - K_t C)AP_{t-1}^{t-1}\\
  P_{T,T-1}^T &=& (I  - K_T C)AP_{T-1}^{T-1}
\end{eqnarray*}

The equation above is the start-up formula for the recursive equation. In order
to derive the recursion,

\begin{eqnarray*}
x_{t-1}^T &=& x_{t-1}^{t-1} + L_{t-1}(x_t^T - Ax_t^{t-1}) \\
-x_{t-1} + x_{t-1}^T - L_{t-1}x_t^T &=& -x_{t-1} + x_{t-1}^{t-1} - L_{t-1}Ax_{t-1}^{t-1}\\
x_{t-1} - x_{t-1}^T + L_{t-1}x_t^T &=& x_{t-1} - x_{t-1}^{t-1} + L_{t-1}Ax_{t-1}^{t-1}\\
\tilde{x}_{t-1}^T + L_{t-1}x_t^T &=& \tilde{x}_{t-1}^{t-1} + L_{t-1}Ax_{t-1}^{t-1}
\end{eqnarray*}

Let's take the last line, subtract 1 from t, take transpose, multiply LHS of the
new equation with LHS of last line above and same with RHS and take expectation
of the final equation.

\begin{eqnarray*}
\tilde{x}_{t-2}^T + L_{t-2}x_{t-1}^T &=& \tilde{x}_{t-2}^{t-2} + L_{t-2}Ax_{t-2}^{t-2}
\end{eqnarray*}

Multiply and take expectation

\begin{eqnarray*}
&& E[ \tilde{x}_{t-1}^T \tilde{x}{_{t-2}^T}' + L_{t-1}x_t^Tx{_{t-1}^T}'L_{t-2}' ] = \\
&& E[ 
  \tilde{x}_{t-1}^{t-1}\tilde{x}{_{t-2}^{t-2}}' + 
  \tilde{x}_{t-1}^{t-1}x{_{t-2}^{t-2}}'A'L_{t-2}' +
  L_{t-1}Ax_{t-1}^{t-1}\tilde{x}{_{t-2}^{t-2}}' +
  L_{t-1}Ax_{t-1}^{t-1}x{_{t-2}^{t-2}}'A'L_{t-2}'
  ]
\end{eqnarray*}

The left-hand side of the equation is
\begin{eqnarray*}
P_{t-1,t-2}^T + L_{t-1}E[x_t^Tx{_{t-1}^T}']L_{t-2}'
\end{eqnarray*}
For RHS's first term, we need definition for $\tilde{x}_{t-1}^{t-1}$. We can
start with $x_t^t$.

\begin{eqnarray*}
x_t^t &=& x_t^{t-1} + K_t(y_t - Cx_t^{t-1})\\
x_t - x_t^t &=& x_t - x_t^{t-1} - K_t(y_t - Cx_t^{t-1})\\
\tilde{x}_t^t  &=& \tilde{x}_t^{t-1} - K_t(Cx_t + \Sigma_w - Cx_t^{t-1})\\
&=& \tilde{x}_t^{t-1} - K_t(C(x_t-x_t^{t-1}) + \Sigma_w)\\
&=& \tilde{x}_t^{t-1} - K_t(C\tilde{x}_t^{t-1} + \Sigma_w)
\end{eqnarray*}

Subtract 1 from t

\begin{eqnarray*}
\tilde{x}_{t-1}^{t-1} &=& \tilde{x}_{t-1}^{t-2} - K_{t-1}(C\tilde{x}_{t-1}^{t-2} + \Sigma_w)
\end{eqnarray*}

We finally have

\begin{eqnarray*}
E[\tilde{x}_{t-1}^{t-1}\tilde{x}{_{t-2}^{t-2}}'] &=&
E[ (\tilde{x}_{t-1}^{t-2} - K_{t-1}(C\tilde{x}_{t-1}^{t-2} + \Sigma_w ))
  \tilde{x}{_{t-2}^{t-2}}'] \\
&=& 
E[ \tilde{x}_{t-1}^{t-2}\tilde{x}{_{t-2}^{t-2}}' - 
  K_{t-1}C\tilde{x}_{t-1}^{t-2}\tilde{x}{_{t-2}^{t-2}}'
]\\
&=& P_{t-1,t-2}^{t-2} - K_{t-1} C P_{t-1,t-2}^{t-2}
\end{eqnarray*}

For RHS's third term, let's define $x_{t-1}^{t-1}$ based on definition of
$\tilde{x}_{t-1}^{t-1}$. 

\begin{eqnarray*}
\tilde{x}_{t-1}^{t-1} = x_{t-1} - x_{t-1}^{t-1}\\
x_{t-1}^{t-1} = x_{t-1}^{t-1} - \tilde{x}_{t-1}^{t-1} 
\end{eqnarray*}

We can use this as

\begin{eqnarray*}
&& E[L_{t-1}Ax_{t-1}^{t-1}\tilde{x}{_{t-2}^{t-2}}'] = \\
&& E[L_{t-1}A(x_{t-1}^{t-1} - \tilde{x}_{t-1}^{t-1} )\tilde{x}{_{t-2}^{t-2}}'] = \\
&& E[L_{t-1}A(x_{t-1} - (\tilde{x}_{t-1}^{t-2} - K_{t-1}(C\tilde{x}_{t-1}^{t-2}
    + \Sigma_w ))) \tilde{x}{_{t-2}^{t-2}}'] = \\
&& E[L_{t-1}Ax_{t-1}\tilde{x}{_{t-2}^{t-2}}' - 
    L_{t-1}A\tilde{x}_{t-1}^{t-2}\tilde{x}{_{t-2}^{t-2}}' +
    L_{t-1}A K_{t-1} C \tilde{x}_{t-1}^{t-2} \tilde{x}{_{t-1}^{t-2}}' +
    L_{t-1}A x_{t-1} \Sigma_w \tilde{x}_{t-2}^{t-2} ] \\
&& = -L_{t-1}AP_{t-1,t-2}^{t-2} + L_{t-1}A K_{t-1}CP_{t-1,t-2}^{t-2}
\end{eqnarray*}

And finally, RHS's fourth term is simply as below;

\begin{eqnarray*}
L_{t-1}A E[x_{t-1}^{t-1}x{_{t-2}^{t-2}}']A'L_{t-2}'
\end{eqnarray*}

Putting all this together, we have

\begin{eqnarray*}
&& P_{t-1,t-2}^T + L_{t-1}E[x_t^Tx{_{t-1}^T}']L_{t-2}' = \\
&& P_{t-1,t-2}^{t-2} - K_{t-1} C P_{t-1,t-2}^{t-2} -
L_{t-1}AP_{t-1,t-2}^{t-2} + 
L_{t-1}A K_{t-1}CP_{t-1,t-2}^{t-2} +\\
&& L_{t-1}A E[x_{t-1}^{t-1}x{_{t-2}^{t-2}}']A'L_{t-2}'
\end{eqnarray*}

We can further simplify this equation. In order to do that, let's remember the
definition of $E[x_t^tx{_{t-1}^t}']$ and $E[x_t^Tx{_{t-1}^T}']$

\begin{eqnarray*}
E[x_t^tx{_{t-1}^t}'] = P_{t,t-1}^t - E[x_tx_{t-1}]
\end{eqnarray*}
and
\begin{eqnarray*}
E[x_t^Tx{_{t-1}^T}'] = AE(x_{t-1}x_{t-2}')A' + A\Sigma_v - P_{t,t-1}^T
\end{eqnarray*}

Let's use this for substitution

\begin{eqnarray*}
&& P_{t-1,t-2}^T + L_{t-1}(A E(x_{t-1}x_{t-2})A' + A\Sigma_v - P_{t,t-1}^T ) L_{t-2}' = \\
&& P_{t-1,t-2}^{t-2} - K_{t-1} C P_{t-1,t-2}^{t-2} -
L_{t-1}AP_{t-1,t-2}^{t-2} + 
L_{t-1}A K_{t-1}CP_{t-1,t-2}^{t-2} + \\
&& L_{t-1}A (P_{t-1,t-2}^{t-2} - E[x_{t-1},x_{t-2}])A'L_{t-2}' 
\end{eqnarray*}

Let's focus on expanding of one term in LHS of above equation

\begin{eqnarray*}
&& L_{t-1}(A E(x_{t-1}x_{t-2})A' + A\Sigma_v - P_{t,t-1}^T ) L_{t-2}' = \\
&&  L_{t-1}A E(x_{t-1}x_{t-2})A' L_{t-2}' + L_{t-1}A\Sigma_vL_{t-2}' 
  - L_{t-1}P_{t,t-1}^TL_{t-2}'
\end{eqnarray*}

Let's expand the last term in RHS 

\begin{eqnarray*}
&& L_{t-1}A (E[x_{t-1},x_{t-2}] - P_{t-1,t-2}^{t-2})A'L_{t-2}' = \\
&& L_{t-1}AE[x_{t-1},x_{t-2}]A'L_{t-2}' - L_{t-1}A P_{t-1,t-2}^{t-2}A'L_{t-2}' 
\end{eqnarray*}

We can see first terms of both LHS and RHS are the same, hence can be
dropped. The simplified equation is

\begin{eqnarray*}
&& P_{t-1,t-2}^T + L_{t-1}A\Sigma_vL_{t-2}' - L_{t-1}P_{t,t-1}^TL_{t-2}' = \\
&& P_{t-1,t-2}^{t-2} - K_{t-1}AP_{t-1,t-2}^{t-2} + L_{t-1}AK_{t-1}CP_{t-1,t-2}^{t-2} - \\
&& L_{t-1}AP_{t-1,t-2}^{t-2}A'L_{t-2}
\end{eqnarray*}

Rearranging

\begin{eqnarray}
&& P_{t-1,t-2}^T = \label{eq10} \\
&& P_{t-1,t-2}^{t-2} - K_{t-1}CP_{t-1,t-2}^{t-2} + \nonumber \\
&& L_{t-1}AK_{t-1}CP_{t-1,t-2}^{t-2} - L_{t-1}AP_{t-1,t-2}^{t-2}A'L_{t-2}' - L_{t-1}A\Sigma_vL_{t-2}'+\nonumber\\
&& L_{t-1}P_{t,t-1}^TL_{t-2}'\nonumber
\end{eqnarray}

Let us simpify this equation further. We will use two shortcuts to do
this. Remember our starting equation for lag-one covariance smoother was

\begin{eqnarray*}
P_{T,T-1}^T &=& (I  - K_T C)AP_{T-1}^{T-1}
\end{eqnarray*}
Then,
\begin{eqnarray*}
P_{t,t-1}^t &=& (I  - K_t C)AP_{t-1}^{t-1}\\
AP_{t-1}^t &=& (I  - K_t C)AP_{t-1}^{t-1}\\
P_{t-1}^t &=& (I  - K_t C)P_{t-1}^{t-1}
\end{eqnarray*}

Another equation we will use is

\begin{eqnarray*}
L_{t-1} = P_{t-1}^{t-1}A'(P_t^{t-1})^{-1}
\end{eqnarray*}

The second line of the Equation \eqref{eq10} can be rewritten as

\begin{eqnarray*}
&& P_{t-1,t-2}^{t-2} - K_{t-1}CP_{t-1,t-2}^{t-2} = \\
&& (I - K_{t-1}C)P_{t-1,t-2}^{t-2} = \\
&& (I - K_{t-1}C) AP_{t-2}^{t-2} = \\
&& (I - K_{t-1}C)P_{t-1}^{t-2}(P_{t-1}^{t-2})^{-1}AP_{t-2}^{t-2} =\\
&& (I - K_{t-1}C)P_{t-1}^{t-2}L_{t-1}' = \\
&& P_{t-1}^{t-1}L_{t-1}'
\end{eqnarray*}

The third line of the Equation \eqref{eq10} can be rewritten as

\begin{eqnarray*}
&& L_{t-1}AK_{t-1}CP_{t-1,t-2}^{t-2} - L_{t-1}AP_{t-1,t-2}^{t-2}A'L_{t-2}' - L_{t-1}A\Sigma_vL_{t-2}'=\\
&& L_{t-1}A(K_{t-1}CP_{t-1,t-2}^{t-2} - P_{t-1,t-2}^{t-2}A'L_{t-2}' - \Sigma_vL_{t-2}')
\end{eqnarray*}

Here we will need 

\begin{eqnarray*}
&& P_{t+1}^t = AP_{t}^tA' + \Sigma_v =\\
&& P_{t+1}^t = P_{t+1,t}^tA' + \Sigma_v
\end{eqnarray*}

which also means

\begin{eqnarray*}
&& P_{t-1}^{t-2} = P_{t-1,t-2}^{t-2}A' + \Sigma_v
\end{eqnarray*}

continuing on the simplification

\begin{eqnarray*}
&& L_{t-1}A(K_{t-1}CP_{t-1,t-2}^{t-2} - (P_{t-1,t-2}^{t-2}A' + \Sigma_v)L_{t-2}')=\\
&& L_{t-1}A(K_{t-1}CP_{t-1,t-2}^{t-2} - P_{t-1}^{t-2}L_{t-2}')=\\
&& L_{t-1}A(K_{t-1}C P_{t-1}^{t-2}(P_{t-1}^{t-2})^{-1} A P_{t-2}^{t-2} - P_{t-1}^{t-2}L_{t-2}')=\\
&& L_{t-1}A(K_{t-1}C P_{t-1}^{t-2}L_{t-2}' - P_{t-1}^{t-2}L_{t-2}')=\\
&& L_{t-1}A(K_{t-1}C P_{t-1}^{t-2} - P_{t-1}^{t-2})L_{t-2}'
\end{eqnarray*}

Putting all the simplified terms together

\begin{eqnarray*}
P_{t-1,t-2}^T &=& P_{t-1}^{t-1}L_{t-2}' + L_{t-1}P_{t,t-1}^TL_{t-2}'
- L_{t-1}AP_{t-1}^{t-1}L_{t-2}'\\
 &=& P_{t-1}^{t-1}L_{t-2}' + L_{t-1}(P_{t,t-1}^T - AP_{t-1}^{t-1})L_{t-2}'
\end{eqnarray*}
which is the final lag-one covariance smoother recursive equation

\end{document}
